Finish equality one step and invariant proof
Change to Z rather than int for time to make lemmas
simpler
Next: combine and push through to full equality

proofs/FEC/DecoderMachine.v
@@ -48,9 +48,33 @@ Qed.
 Definition sint64 (i: int64) : S64.I.int :=
   S64.I.mkint (Int64.intval i) (Int64.intrange i).
 
+Lemma s64_inj (i1 i2: S64.I.int):
+  S64.I.unsigned i1 = S64.I.unsigned i2 ->
+  i1 = i2.
+Proof.
+  move=> Heq. 
+  by rewrite -(S64.I.repr_unsigned i1) -(S64.I.repr_unsigned i2) Heq.
+Qed.
+
+Lemma sint64_repr (z: Z):
+  sint64 (Int64.repr z) = S64.I.repr z.
+Proof.
+  rewrite /sint64/=.
+  eapply eq_trans.
+  2: apply s64_inj.
+  reflexivity. by [].
+Qed.
+
 Section Machine.
 
-Definition create_block_with_fec_packet_m (p: fpacket) (time : int) : 
+(*Hmm, let's think about this - can have time as Z because all
+  operations are in terms of Int.repr time - but I think we
+  want the _m versions with Znth because otherwise we need to
+  prove in VST proof
+  TODO: make sure*)
+
+
+Definition create_block_with_fec_packet_m (p: fpacket) (time : Z) : 
   block :=
   let k := fd_k p in
   let h := fd_h p in
@@ -58,9 +82,19 @@ Definition create_block_with_fec_packet_m (p: fpacket) (time : int) :
     (Int.unsigned (Int.repr (Z.of_nat (fd_blockIndex p)))) 
     (zseq (k + h) None) (Some p) in
   mk_blk (fd_blockId p) (sublist 0 k allPackets) 
-    (sublist k (k+h) allPackets) k h false (Int.unsigned time).
+    (sublist k (k+h) allPackets) k h false time.
 
-Definition create_block_with_packet_black_m (p: fpacket) (time: int) : block * list packet :=
+Lemma create_m_eq (p: fpacket) (time: Z) :
+  (Z.of_nat (fd_blockIndex p) <= Int.max_unsigned) ->
+  create_block_with_fec_packet_m p time =
+  create_block_with_fec_packet p time.
+Proof.
+  move=> Hidx. 
+  rewrite /create_block_with_fec_packet_m/create_block_with_fec_packet.
+  by rewrite Int.unsigned_repr; try rep_lia.
+Qed.
+
+Definition create_block_with_packet_black_m (p: fpacket) (time: Z) : block * list packet :=
   let new_block := create_block_with_fec_packet_m p time in
   let packets  := (if (fd_isParity p) then nil else 
     [:: p_packet p ]) ++
@@ -70,6 +104,21 @@ Definition create_block_with_packet_black_m (p: fpacket) (time: int) : block * l
     new_block <| black_complete := true |> else new_block in
   (marked_block, packets).
 
+Lemma create_black_m_eq (p: fpacket) (time: Z) : 
+  (Z.of_nat (fd_blockIndex p) <= Int.max_unsigned) ->
+  (0 <= fd_k p <= Int.max_unsigned) ->
+  create_block_with_packet_black_m p time =
+  create_block_with_packet_black p time.
+Proof.
+  move=> Hidx Hk.
+  rewrite /create_block_with_packet_black_m
+    /create_block_with_packet_black.
+  rewrite /Int.eq Int.unsigned_repr=>[|//].
+  rewrite Int.unsigned_one /zeq.
+  by case: Z.eq_dec=> [Heq/=| Hneq/=];
+  rewrite create_m_eq.
+Qed.
+
 (*2. add packet to block*)
 Definition add_fec_packet_to_block_m (p: fpacket) (b: block) : block :=
   let new_packets := upd_Znth 
@@ -77,6 +126,15 @@ Definition add_fec_packet_to_block_m (p: fpacket) (b: block) : block :=
     (data_packets b ++ parity_packets b) (Some p) in
   b <| data_packets := sublist 0 (blk_k b) new_packets |> 
       <| parity_packets := sublist (blk_k b) (blk_k b + blk_h b) new_packets |>.
+
+Lemma add_m_eq (p: fpacket) (b: block) :
+  (Z.of_nat (fd_blockIndex p) <= Int.max_unsigned) ->
+  add_fec_packet_to_block_m p b =
+  add_fec_packet_to_block p b.
+Proof.
+  move=> Hidx. rewrite /add_fec_packet_to_block_m/add_fec_packet_to_block.
+  by rewrite !Int.unsigned_repr //; rep_lia.
+Qed.
 
 Definition add_packet_to_block_black_m (p: fpacket) (b: block) : block * list packet :=
   (*NOTE: we still must add the packet even if the block is complete
@@ -93,6 +151,16 @@ Definition add_packet_to_block_black_m (p: fpacket) (b: block) : block * list pa
       new_block <| black_complete := true |> else new_block in
     (marked_block, packets).
 
+Lemma add_black_m_eq (p: fpacket) (b: block) :
+  (Z.of_nat (fd_blockIndex p) <= Int.max_unsigned) ->
+  add_packet_to_block_black_m p b =
+  add_packet_to_block_black p b.
+Proof.
+  move=> Hidx.
+  rewrite /add_packet_to_block_black_m/add_packet_to_block_black.
+  by rewrite !add_m_eq.
+Qed.
+
 Variable threshold : int.
 
 (*Once again, will have more efficient version like C code, 
@@ -100,8 +168,8 @@ Variable threshold : int.
 (*TODO: is it nontrivial to prove equivalence? Probably not
   because we can easily prove everything is within required bounds*)
 (*TODO: use from before?*)
-Definition block_notin_packet block packet : bool :=
-    ~~ (packet_in_block packet block).
+(*Definition block_notin_packet block packet : bool :=
+    ~~ (packet_in_block packet block).*)
 
 (*NOTE: We are changing the code to use 64 bit integers and thus
   Int64 comparison operations. Then, we can assume that all
@@ -113,21 +181,22 @@ Definition block_notin_packet block packet : bool :=
   the stronger conditions for ensuring packet recovery.
   TOOD: write this somewhere
   *)
-
+(*I think: shouldn't need this or any: still store Z, just
+  do comparisons on Int.repr time*)
 (*The check to update the time*)
-Fixpoint upd_time_m (time: int) (curr: fpacket) (blocks: list block) :
-  int := 
+Fixpoint upd_time_m (time: Z) (curr: fpacket) (blocks: list block) :
+  Z := 
   match blocks with
-  | nil => Int.add time Int.one
+  | nil => time + 1 (*Int.add (Int.repr time) Int.one*)
   | bl :: tl =>
     let currSeq := Int64.repr (Z.of_nat (fd_blockId curr)) in
     let blkid := Int64.repr (Z.of_nat (blk_id bl)) in
-    if Int64.eq currSeq blkid then
+    if S64.seq_eq (sint64 currSeq) (sint64 blkid) then
       if (block_notin_packet bl curr) 
-      then Int.add time Int.one 
+      then time + 1 (*Int.add (Int.repr time) Int.one*)
       else time
     else if S64.seq_lt (sint64 currSeq) (sint64 blkid) 
-      then Int.add time Int.one
+      then time + 1 (*Int.add time Int.one*)
     else upd_time_m time curr tl
   end.
 
@@ -140,31 +209,31 @@ Definition seq_leq (i1 i2: int) : bool :=
 (*Hmm, what happens if time wraps around? - maybe for this 
 we should do sequence number comparison because times will 
 always be within threshold?*)
-Definition not_timed_out_m: int -> block -> bool := fun currTime =>
-  (fun b => S32.seq_leq (sint currTime) 
+Definition not_timed_out_m: Z -> block -> bool := fun currTime =>
+  (fun b => S32.seq_leq (sint (Int.repr currTime)) 
     (sint (Int.add (Int.repr(black_time b)) threshold))).
 
 Fixpoint update_dec_state_m (blocks: list block) (curr: fpacket)
-  (time: int) : list block * list packet:=
+  (time: Z) : list block * list packet:=
 match blocks with
-| nil => let t := create_block_with_packet_black_m curr time in 
+| nil => let t := create_block_with_packet_black curr time in 
     ([:: t.1], t.2)
 | bl :: tl =>
   let currSeq := Int64.repr (Z.of_nat (fd_blockId curr)) in
   let blkid := Int64.repr (Z.of_nat (blk_id bl)) in
-  if Int64.eq currSeq blkid then
+  if S64.seq_eq (sint64 currSeq) (sint64 blkid) then
     let t := add_packet_to_block_black_m curr bl in
     (t.1 :: tl, t.2)
     else if S64.seq_lt (sint64 currSeq) (sint64 blkid) then
-    let t := create_block_with_packet_black_m curr time in 
+    let t := create_block_with_packet_black curr time in 
       (t.1 :: blocks, t.2)
   else 
     let t := update_dec_state_m tl curr time
     in (bl :: t.1, t.2)
 end.
 
-Definition decoder_one_step_m (blocks: list block) curr (time : int) :
-list block * list packet * int :=
+Definition decoder_one_step_m (blocks: list block) curr (time : Z) :
+list block * list packet * Z :=
 (*First, we process timeouts; this covers the case when the packet
   which makes the block timeout is the kth packet; we should not
   recover this block (it makes our invariants much harder).*)
@@ -175,17 +244,17 @@ let t := update_dec_state_m blks curr tm in
 
 Definition decoder_multiple_steps_m
 (prev_packs packs: list fpacket)
-(state: list block) (sent: list packet) (time: int) :
-list block * list packet * int * list fpacket :=
-foldl (fun (acc: list block * list packet * int * list fpacket) 
+(state: list block) (sent: list packet) (time: Z) :
+list block * list packet * Z * list fpacket :=
+foldl (fun (acc: list block * list packet * Z * list fpacket) 
   (p: fpacket) =>
   let t := decoder_one_step_m acc.1.1.1 p acc.1.2 in
   (t.1.1, acc.1.1.2 ++ t.1.2, t.2, acc.2 ++ [:: p])) 
 (state, sent, time, prev_packs) packs.
 
 Definition decoder_all_steps_m (received: list fpacket) :
-(list block * list packet * int) :=
-(decoder_multiple_steps_m nil received nil nil Int.zero).1.
+(list block * list packet * Z) :=
+(decoder_multiple_steps_m nil received nil nil 0).1.
 
 (*Now we have to prove equivalence. This means we have to show that
   every comparison between unsigned ints occurs between those
@@ -221,11 +290,12 @@ Definition dec_machine_invar (blks: seq block)
   (time: Z) : Prop :=
   (*All black times are no more than [threshold] behind the
     current time*)
-  (forall (b: block), b \in blks -> 
-    (Z.abs (black_time b - time) <= Int.unsigned threshold)%Z) /\
+  (forall (b: block), b \in blks ->
+    (0 <= time - (black_time b) <= Int.unsigned threshold)%Z) /\
+    (*(Z.abs (black_time b - time) <= Int.unsigned threshold)%Z) /\*)
   (*All block ids are smaller than 2^61-1*)
   (forall (b: block), b \in blks -> 
-    blk_id b < Z.to_nat Int64.half_modulus).
+    Z.of_nat (blk_id b) < Int64.half_modulus)%Z.
 
 (*First, show this invariant implies equality*)
 
@@ -235,29 +305,79 @@ Local Definition convert_tuple {A B: Type} (x: (A * B * Z)) :
   | (a, b, z) => (a, b, Int.repr z)
   end.
 
-Lemma decoder_one_step_m_eq_aux (blks: seq block) (time: Z) 
-  (curr: fpacket) :
-  p_seqNum curr < Z.to_nat Int64.half_modulus ->
-  (Int.unsigned threshold < Int.half_modulus / 2)%Z ->
-  dec_machine_invar blks time ->
-  (decoder_one_step_m blks curr (Int.repr time)).1 =
-  (decoder_one_step (Int.unsigned threshold) blks curr time).1 /\
-  Int.unsigned (decoder_one_step_m blks curr (Int.repr time)).2 =
-  ((decoder_one_step (Int.unsigned threshold) blks curr time).2).
+(*Helpful here*)
+Lemma znat_eq (n1 n2 : nat) :
+  Z.eqb (Z.of_nat n1) (Z.of_nat n2) = (n1 == n2).
 Proof.
-  move=> Hcurr Hthreshlt [Hthresh Hallid].
-  rewrite /decoder_one_step_m/decoder_one_step/=.
-  have Htime1: Int.unsigned (upd_time_m (Int.repr time) curr blks) = 
+  case: (Z.of_nat n1 =? Z.of_nat n2)%Z /Z.eqb_spec => [Heq | Hneq];
+  symmetry; apply /eqP; lia.
+Qed. 
+
+Lemma znat_lt (n1 n2: nat):
+  Z.ltb (Z.of_nat n1) (Z.of_nat n2) = (n1 < n2).
+Proof.
+  case: ((Z.of_nat n1 <? Z.of_nat n2)%Z) /Z.ltb_spec => [Hlt | Hge];
+  symmetry; apply /ltP; lia.
+Qed.
+
+(*TODO: dont need anymore, but we will need in VST proofs*)
+Lemma int_add_one (z: Z):
+  Int.add (Int.repr z) Int.one = Int.repr (z + 1).
+Proof.
+  apply Endian.int_unsigned_inj. (*TODO: move*)
+  by rewrite /Int.add/Int.one !Int.unsigned_repr_eq -Zplus_mod.
+Qed.
+
+(*TODO: move*)
+Lemma upd_time_bound (time: Z) (curr: fpacket) (blks: seq block) :
+  (time <= upd_time time curr blks <= time + 1)%Z.
+Proof.
+  elim: blks => [/= | b btl IH /=]; try lia.
+  case: (fd_blockId curr == blk_id b).
+  - by case: (block_notin_packet b curr); lia.
+  - by case: (fd_blockId curr < blk_id b)%N; lia.
+Qed.
+
+Variable thresh_bound: 
+  (Int.unsigned threshold < Int.half_modulus / 2)%Z.
+
+Lemma decoder_one_step_m_eq (blks: seq block) (time: Z) 
+  (curr: fpacket) :
+  (Z.of_nat (fd_blockId curr) < Int64.half_modulus)%Z ->
+  (Z.of_nat (fd_blockIndex curr) <= Int.max_unsigned)%Z ->
+  (0 <= fd_k curr < Int.modulus)%Z ->
+  dec_machine_invar blks time ->
+  decoder_one_step_m blks curr time =
+  decoder_one_step (Int.unsigned threshold) blks curr time.
+Proof.
+  move=> Hcurr Hidx Hkbound [Hthresh Hallid].
+  rewrite /decoder_one_step_m/decoder_one_step/decoder_one_step_gen/=.
+  have Htime: upd_time_m time curr blks = 
     upd_time time curr blks. {
-      admit.
+    rewrite {Hthresh}. move: Hallid. elim: blks => [_ //=|b btl IH Hallid /=].
+      have Hbound: (z_abs_diff 
+      (Z.of_nat (fd_blockId curr)) (Z.of_nat (blk_id b)) <
+        S64.I.half_modulus)%Z. {
+        (*Easy: both are smaller than half_modulus*)
+        rewrite /z_abs_diff.
+        move: Hallid => /(_ _ (mem_head _ _)).
+        have->:S64.I.half_modulus = Int64.half_modulus by [].
+        rep_lia.
+      }
+      rewrite !sint64_repr S64.seq_eq_eq. 
+      + rewrite znat_eq.
+        case: (fd_blockId curr == blk_id b) /eqP => Hbcurr.
+        * by case: (block_notin_packet b curr).
+        * rewrite S64.seq_lt_lt // znat_lt.
+          case: (fd_blockId curr < blk_id b) =>//. 
+          apply IH => b' Hinb'. apply Hallid. 
+          by rewrite in_cons Hinb' orbT.
+      + have: (S64.I.half_modulus < S64.I.modulus)%Z by []. lia.
   }
-  have Htime: upd_time_m (Int.repr time) curr blks = 
-    Int.repr (upd_time time curr blks) by
-    rewrite -Htime1 Int.repr_unsigned.
-  split=>[|//].
+  f_equal=>//.
   rewrite Htime.
   have->: [seq x <- blks | 
-    not_timed_out_m (Int.repr (upd_time time curr blks)) x] =
+    not_timed_out_m (upd_time time curr blks) x] =
     [seq x <- blks | 
     not_timed_out (Int.unsigned threshold) (upd_time time curr blks) x]. 
     {
@@ -272,35 +392,136 @@ Proof.
     - (*Here, use fact that upd_time increases by at most 1
         and that before, all were within threshold. So here,
         should be ok*)
-        (*see*)
-        have: (time <= upd_time time curr blks <= time + 1)%Z by admit.
+        have:=(upd_time_bound time curr blks).
         rewrite /z_abs_diff.
         move: Hthresh => /(_ b Hinb).
         have->: S32.I.half_modulus = Int.half_modulus by [].
-        (*i think this is true with the additional /2 in the half
-        modulus but TODO: and see if we need the bound*)
+        move: thresh_bound=>/=. rep_lia.
+    }
+    move: (upd_time time curr blks) => tm.
+    have: forall b, b \in 
+    [seq x <- blks | not_timed_out (Int.unsigned threshold) tm x] ->
+    (Z.of_nat (blk_id b) < Int64.half_modulus)%Z. {
+      move=> b'. rewrite mem_filter => /andP[_ Hinb]. by apply Hallid.
+    }
+    rewrite {Htime Hthresh Hallid}.
+    move: ([seq x <- blks | not_timed_out (Int.unsigned threshold) tm x] ) => bs.
+    (*Now show equality - similar to time proof above*)
+    elim: bs => [ _ // | b btl IH Hallid //=].
+    have Hbound: (z_abs_diff 
+      (Z.of_nat (fd_blockId curr)) (Z.of_nat (blk_id b)) <
+        S64.I.half_modulus)%Z. {
+        (*Easy: both are smaller than half_modulus*)
+        rewrite /z_abs_diff.
+        move: Hallid => /(_ _ (mem_head _ _)).
+        have->:S64.I.half_modulus = Int64.half_modulus by [].
         rep_lia.
+      }
+    rewrite !sint64_repr S64.seq_eq_eq.
+    - rewrite znat_eq.
+      case: (fd_blockId curr == blk_id b) /eqP => [Heq|Hneq].
+      + by rewrite add_black_m_eq.
+      + rewrite S64.seq_lt_lt // znat_lt.
+        case: (fd_blockId curr < blk_id b) =>//.
+        rewrite IH // => b' Hinb'. 
+        apply Hallid. 
+        by rewrite in_cons Hinb' orbT.
+    - have: (S64.I.half_modulus < S64.I.modulus)%Z by []. lia.
+Qed.
+
+(*TODO; move*)
+Lemma add_black_m_id (curr: fpacket) (b: block) :
+  blk_id (add_packet_to_block_black_m curr b).1 =
+  blk_id b.
+Proof.
+  rewrite /add_packet_to_block_black_m.
+  case: (black_complete b)=>//=.
+  by case: (recoverable (add_fec_packet_to_block_m curr b)).
+Qed.
+
+
+(*Now, we have to prove preservation of the invariant.
+  We use the equality lemma to help (TODO: maybe)*)
+(*Here, we prove for the non-machine version, then use
+  the previous lemma to show the invariant for the machine one*)
+Lemma decoder_m_invar_one_step (blks: seq block) (time: Z) 
+  (curr: fpacket) :
+  (Z.of_nat (fd_blockId curr) < Int64.half_modulus)%Z ->
+  dec_machine_invar blks time ->
+  dec_machine_invar (decoder_one_step (Int.unsigned threshold) 
+    blks curr time).1.1
+    (decoder_one_step (Int.unsigned threshold) blks curr time).2.
+Proof.
+  rewrite /dec_machine_invar => Hid [Hthresh Hallid].
+  (*First try to do without lemma (so we dont need more
+    assumptions), otherwise, do with lemma - may be easier*)
+  rewrite /decoder_one_step/=.
+  split.
+  - move=> b.
+
+    have: forall b, b \in [seq x <- blks
+    | not_timed_out (Int.unsigned threshold)
+        (upd_time time curr blks) x] ->
+    ((upd_time time curr blks) <= 
+      black_time b + Int.unsigned threshold)%Z /\
+      (0 <= time - black_time b)%Z. {
+      move=> b'. rewrite mem_filter => /andP. 
+      rewrite /not_timed_out => [[]] /Z.leb_spec0 Hle Hinb'.
+      move: Hthresh => /(_ _ Hinb').
+      lia.
+    }
+    have:=(upd_time_bound time curr blks).
+    move: (upd_time time curr blks) => tm.
+    move: [seq x0 <- blks | not_timed_out (Int.unsigned threshold) tm x0] => bs.
+    rewrite {Hthresh Hallid blks}.
+    elim: bs => [// Htm Hallid /=|bhd btl IH Htm Hallid /=].
+    + rewrite in_cons orbF => /eqP ->.
+      case: Z.eq_dec=>//=; rep_lia.
+    + have Hhd: (0 <= tm - black_time bhd <= Int.unsigned threshold)%Z by
+      move: Hallid => /( _ _ (mem_head _ _)); rep_lia.
+      have Htl: forall b, b \in btl ->
+      (0 <= tm - black_time b <= Int.unsigned threshold)%Z. {
+        move=> b' Hinb.
+        move: Hallid => /(_ b'). rewrite in_cons Hinb orbT => /(_ isT).
         rep_lia.
-
-    (*rewrite -{1}(Int.repr_unsigned threshold).*)
-    rewrite !sint_repr S32.seq_leq_leq.
-    (*TODO: why is this true? Start here and think about wraparound*)
-    
-    !Int.unsigned_repr_eq.
-    Search Zmod (_ + _)%Z.
-    Search ((?x + ?y)%Z mod ?z).
-    
-    S32.seq_leq_leq.
-    
-    
-    /seq_leq.
-    
-
-    Print seq_leq.
-    Search (filter ?f ?l = filter ?g ?l).
-  }
-
-
-(*We prove both that this invariant is preserved and that
-  this invariant implies equality*)
-
+      }
+    case: (fd_blockId curr == blk_id bhd).
+      * rewrite in_cons => /orP[/eqP -> | Hinb].
+        -- by rewrite add_black_time.
+        -- by apply Htl.
+      * case: (fd_blockId curr < blk_id bhd)=>/=.
+        -- case: Z.eq_dec=>/= Hk1;
+          rewrite !in_cons => /orP[/eqP -> /= | /orP[/eqP -> | Hinb]];
+            try rep_lia; by apply Htl.
+        -- rewrite in_cons => /orP[/eqP -> // | Hinb].
+          apply IH =>//. move=> b' Hinb'. apply Hallid.
+          by rewrite in_cons Hinb' orbT.
+  - (*This invariant is a bit easier*)
+     have: forall b, b \in 
+     [seq x <- blks
+     | not_timed_out (Int.unsigned threshold)
+         (upd_time time curr blks) x] ->
+    (Z.of_nat (blk_id b) < Int64.half_modulus)%Z. {
+      move=> b'. rewrite mem_filter=> /andP[_ Hinb'].
+      by apply Hallid.
+    }
+    rewrite {Hthresh Hallid}.
+    move: (upd_time time curr blks) => tm.
+    move: [seq x <- blks | not_timed_out (Int.unsigned threshold) tm x] => bs.
+    elim: bs => [Hallid b/=|b bs IH Hallid /=].
+    + rewrite in_cons orbF => /eqP ->. by case: Z.eq_dec => Hk1//=.
+    + move=> b'.
+      case: (fd_blockId curr == blk_id b).
+      * rewrite in_cons => /orP[/eqP -> | Hinb']; last by
+        apply Hallid; rewrite in_cons Hinb' orbT.
+        rewrite add_black_id. apply Hallid. by rewrite mem_head.
+      * case: (fd_blockId curr < blk_id b).
+        -- rewrite in_cons => /orP[/eqP -> | Hinb']; last by apply Hallid.
+          by case: Z.eq_dec.
+        -- rewrite in_cons => /orP[/eqP -> | Hin]; first by apply Hallid;
+          rewrite mem_head. apply IH=>//.
+          move=> b'' Hinb''. apply Hallid. by rewrite in_cons Hinb'' orbT.
+Qed.
+        
+(*TODO: connect lemmas to show full preservation of
+  invariant + prove full equality*)
